start proving soundness

Clean/Gadgets/BLAKE3/BLAKE3G.lean
@@ -55,15 +55,6 @@ def main (a b c d : Fin 16) (input : Var Inputs (F p)) : Circuit (F p) (Var BLAK
                     |>.set d state_d
   return state
 
-
-def c := main (p:=p_babybear) 0 1 2 3 {
-  state := default,
-  x := default,
-  y := default
-}
-#eval! c.operations.local_length
-#eval! c.output
-
 instance elaborated (a b c d : Fin 16): ElaboratedCircuit (F p) Inputs BLAKE3State where
   main := main a b c d
   local_length _ := 112
@@ -76,6 +67,53 @@ instance elaborated (a b c d : Fin 16): ElaboratedCircuit (F p) Inputs BLAKE3Sta
   local_length_eq _ n := by
     simp [main, circuit_norm, Xor32.circuit, Addition32.circuit, Rotation32.circuit,
       Xor32.elaborated, Addition32.elaborated, Rotation32.elaborated]
+
+def assumptions (input : Inputs (F p)) :=
+  let { state, x, y } := input
+  state.is_normalized ∧ x.is_normalized ∧ y.is_normalized
+
+def spec (a b c d : Fin 16) (input : Inputs (F p)) (out: BLAKE3State (F p)) :=
+  let { state, x, y } := input
+  out.value = g state.value a b c d x.value y.value ∧ out.is_normalized
+
+theorem soundness (a b c d : Fin 16) : Soundness (F p) (elaborated a b c d) assumptions (spec a b c d) := by
+  intro i0 env ⟨state_var, x_var, y_var⟩ ⟨state, x, y⟩ h_input h_normalized h_holds
+  dsimp [circuit_norm, subcircuit_norm, elaborated, main, spec,
+    Addition32.circuit, Addition32.elaborated,
+    Xor32.circuit, Xor32.elaborated,
+    Rotation32.circuit, Rotation32.elaborated,
+  ] at h_holds
+  simp [circuit_norm, elaborated, main, spec]
+  dsimp [assumptions] at h_normalized
+
+  -- normalize offsets
+  ring_nf at h_holds ⊢
+  obtain ⟨c1, c2, c3, c4, c5, c6, c7, c8, c9, c10, c11, c12, c13, c14⟩ := h_holds
+
+  -- give names to intermediate variables for clarity
+  set tmp1 : U32 (Expression (F p)) := ⟨var ⟨i0⟩, var ⟨2 + i0⟩, var ⟨4 + i0⟩, var ⟨6 + i0⟩⟩
+  set state_a1 : U32 (Expression (F p)) := ⟨var ⟨8 + i0⟩, var ⟨10 + i0⟩, var ⟨12 + i0⟩, var ⟨14 + i0⟩⟩
+  set tmp2 := var_from_offset U32 (16 + i0)
+  set state_d1 : U32 (Expression (F p)) := ⟨var ⟨20 + i0⟩, var ⟨22 + i0⟩, var ⟨24 + i0⟩, var ⟨26 + i0⟩⟩
+  set tmp3 := var_from_offset U32 (28 + i0)
+  set state_c1 : U32 (Expression (F p)) := ⟨var ⟨32 + i0⟩, var ⟨34 + i0⟩, var ⟨36 + i0⟩, var ⟨38 + i0⟩⟩
+  set tmp4 := var_from_offset U32 (40 + i0)
+  set state_b1 := var_from_offset U32 (52 + i0)
+
+  set tmp5 : U32 (Expression (F p)) := ⟨var ⟨56 + i0⟩, var ⟨58 + i0⟩, var ⟨60 + i0⟩, var ⟨62 + i0⟩⟩
+  set state_a2 : U32 (Expression (F p)) := ⟨var ⟨64 + i0⟩, var ⟨66 + i0⟩, var ⟨68 + i0⟩, var ⟨70 + i0⟩⟩
+  set tmp6 := var_from_offset U32 (72 + i0)
+  set state_d2 := var_from_offset U32 (84 + i0)
+  set state_c2 : U32 (Expression (F p)) := ⟨var ⟨88 + i0⟩, var ⟨90 + i0⟩, var ⟨92 + i0⟩, var ⟨94 + i0⟩⟩
+  set tmp7 := var_from_offset U32 (96 + i0)
+  set state_b2 := var_from_offset U32 (108 + i0)
+
+
+
+  simp [circuit_norm, eval, Expression.eval] at c1
+  constructor
+  · sorry
+  · sorry
 
 
 
